# 4-3 Solving recurrences with a change of variables

> Sometimes, a little algebraic manipulation can make an unknown recurrence similar to one you have seen before. Letâ€™s solve the recurrence
>
> $T(n)=2T(\sqrt{n})+\Theta(\lg n)$
>
> by using the change-of-variables method.
>
> **a**. Define $m=\lg n$ and $S(m)=T(2^m)$. Rewrite recurrence (4.25) in terms of m and $S(m)$.
>
> **b**. Solve your recurrence for $S(m)$.
>
> **c**. Use your solution for $S(m)$ to conclude that $T(n)=\Theta(\lg n\lg\lg n)$.
>
> **d**. Sketch the recursion tree for recurrence (4.25), and use it to explain intuitively why the solution is $T(n)=\Theta(\lg n \lg\lg n)$.
>
> Solve the following recurrences by changing variables:
>
> **e**. $T(n)=2T(\sqrt{n})+\Theta(1)$.
>
> **f**. $T(n)=3T(\sqrt[3]{n})+\Theta(n)$.
