# 3-1 Asymptotic behavior of polynomials

> Let
>
> $$
> P(n) = \sum_{i=0}^d a_i n^i,
> $$
>
> where $a_d > 0$, be a degree-d polynomial in n, and let k be a constant. Use the definitions of the asymptotic notations to prove the following properties.
>
> **a**. if $k \geq d$, then $p(n)=O(n^k)$
>
> **b**. if $k \leq d$, then $p(n)=\Omega(n^k)$
>
> **c**. if $k =d$, then $p(n)=\Theta(n^k)$
>
> **d**. if $k > d$, then $p(n)=o(n^k)$
>
> **e**. if $k < d$, then $p(n)=\omega(n^k)$

## **a**

To prove $p(n)=O(n^k)$, we only need to prove:

$$
\begin{aligned}
    \sum_{i=0}^{d}a_in^i \leq cn^k (\text{ for }n \geq n_0)\cr
\end{aligned}
$$

Which is implied by

$$
\begin{aligned}
    c \geq \sum_{i=0}^da_in^{i-k}  (\text{ for }n \geq n_0)\cr
\end{aligned}
$$
since $\sum_{i=0}^{d}a_i \geq \sum_{i=0}^da_in^{i-k} (\text{ for }n \geq 1)$

$\text{choose } c = \sum_{i=0}^{d}a_i$ and $n_0 = 1$ satisfies.

- Tips: the description of $n>n_0$ and $c$ will be omitted next time.

## **b**

We only need to prove:

$$
    \sum_{i=0}^{d}a_in^i \geq cn^k
$$

which is implied by:

$$
\begin{aligned}
    c \leq \sum_{i=0}^da_in^{i-k}\cr
    c=a_d \leq \sum_{i=0}^da_in^{i-k}\cr
    n_0=1
\end{aligned}
$$

## **c**

We only need to prove:

$$
    c_1n^d\leq \sum_{i=0}^{d}a_in^i \leq c_2n^{d}
$$

which is implied by:

$$
\begin{aligned}
    c_1 \leq \sum_{i=0}^da_in^{i-d} \leq c_2\cr
    c_1=a_d \leq \sum_{i=0}^da_in^{i-d} \leq \sum_{i=0}^{d} a_i=c_2\cr
    n_0=1
\end{aligned}
$$

## **d**

We only need to prove:
$$
\begin{aligned}
    \forall c >0,\exist n_0 \text{ satisfies: }\cr
    \sum_{i=0}^{d} a_i n^i < cn^k (\text{ for } n > n_0)\cr
    \impliedby c > \sum_{i=0}^{d} a_in^{i-k}\cr
    \text{since }\sum_{i=0}^{d} a_in^{d-k} \geq \sum_{i=0}^{d} a_in^{i-k}\cr
    n_0=\sqrt[d-k]{\frac {c} {\sum_{i=0}^d a_i}}
\end{aligned}
$$

## **e**

We only need to prove:
$$
\begin{aligned}
    \forall c >0,\exist n_0 \text{ satisfies: }\cr
    \sum_{i=0}^{d} a_in^i > cn^k (\text{ for }n>n_0)\cr
    \impliedby c < \sum_{i=0}^{d} a_in^{i-k}\cr
    \text{since } a_d n^{d-k} \leq \sum_{i=0}^{d} a_in^{i-k}\cr
    n_0=\sqrt[d-k]{\frac {c} {a_d}}
\end{aligned}
$$
